Proof of BankClerk__Transfer except for overflow reasoning

src/program_proof/lockservice/bank_proof.v
@@ -22,7 +22,7 @@ Record bank_names := BankGN {
 Class bankG Σ := BankG {
   bank_ls :> lockserviceG Σ;
   bank_ks :> kvserviceG Σ;
-  bank_logBalG :> mapG Σ u64 u64
+  (* bank_logBalG :> mapG Σ u64 u64 *)
 }.
 
 Section bank_proof.
@@ -36,10 +36,13 @@ Context `{acc1:u64, acc2:u64, bal_total:Z}. (* Account names and total balance f
 Definition kv_gn γ := γ.(bank_ks_names).(ks_kvMapGN).
 Definition log_gn γ := γ.(bank_logBalGN).
 
+Definition bankPs γ := λ k, (∃v, k [[kv_gn γ]]↦v ∗ k [[log_gn γ]]↦v)%I.
+
 (* TODO: consider making is_*server part of own_*clerk *)
 Definition own_bank_clerk (bank_ck:loc) γ : iProp Σ :=
   ∃ (lck kck ls_srv ks_srv:loc), 
-  "#Hls" ∷ is_lockserver ls_srv γ.(bank_ls_names) (Ps:=λ k, (∃v, k [[kv_gn γ]]↦v ∗ k [[log_gn γ]]↦v) )∗
+  "%" ∷ ⌜acc1 ≠ acc2⌝ ∗
+  "#Hls" ∷ is_lockserver ls_srv γ.(bank_ls_names) (Ps:=bankPs γ) ∗
   "#Hks" ∷ is_kvserver ks_srv γ.(bank_ks_names) ∗
   "Hlck_own" ∷ own_clerk #lck ls_srv γ.(bank_ls_names).(ls_rpcGN) ∗
   "Hkck_own" ∷ own_kvclerk kck ks_srv γ.(bank_ks_names).(ks_rpcGN) ∗
@@ -53,15 +56,43 @@ Definition own_bank_clerk (bank_ck:loc) γ : iProp Σ :=
   "Hacc2_is_lock" ∷ lockservice_is_lock γ.(bank_ls_names) acc2
 .
 
-Check bal_total.
-
 Definition bank_inv γ : iProp Σ :=
   ∃ (bal1 bal2:u64),
-  "HlogBalCtxl" ∷ map_ctx (log_gn γ) 1 ({[ acc1:=bal1 ]} ∪ {[ acc2:=bal2 ]}) ∗
-  ⌜(int.Z bal1 + int.Z bal2 = bal_total)%Z⌝
+  "HlogBalCtx" ∷ map_ctx (log_gn γ) 1 ({[ acc1:=bal1 ]} ∪ {[ acc2:=bal2 ]}) ∗
+  "%" ∷ ⌜(int.Z bal1 + int.Z bal2 = bal_total)%Z⌝
   .
 
 Definition bankN := nroot .@ "bank".
+
+Lemma acquire_two_spec (lck lsrv :loc) (ln1 ln2:u64) γ:
+let γrpc := γ.(bank_ls_names).(ls_rpcGN) in
+{{{
+     is_lockserver lsrv γ.(bank_ls_names) (Ps:=bankPs γ) ∗
+     own_clerk #lck lsrv γrpc
+}}}
+  acquire_two #lck #ln1 #ln2
+{{{
+     RET #(); own_clerk #lck lsrv γrpc ∗
+     bankPs γ ln1 ∗
+     bankPs γ ln2
+}}}.
+Proof.
+Admitted.
+
+Lemma release_two_spec (lck lsrv :loc) (ln1 ln2:u64) γ:
+let γrpc := γ.(bank_ls_names).(ls_rpcGN) in
+{{{
+     is_lockserver lsrv γ.(bank_ls_names) (Ps:=bankPs γ) ∗
+     bankPs γ ln1 ∗
+     bankPs γ ln2 ∗
+     own_clerk #lck lsrv γrpc
+}}}
+  release_two #lck #ln1 #ln2
+{{{
+     RET #(); own_clerk #lck lsrv γrpc
+}}}.
+Proof.
+Admitted.
 
 Lemma Bank__SimpleTransfer_spec (bck:loc) (amount:u64) γ :
 {{{
@@ -85,6 +116,52 @@ Proof.
   wp_lam. (* We just use the helper function in-line *)
   wp_pures.
   wp_loadField.
+  wp_apply (acquire_two_spec with "[$Hlck_own $Hls]").
+  iIntros "(Hlck_own & Hacc1_unlocked & Hacc2_unlocked)".
+  iDestruct "Hacc1_unlocked" as (bal1) "(Hacc1_phys & Hacc1_log)".
+  iDestruct "Hacc2_unlocked" as (bal2) "(Hacc2_phys & Hacc2_log)".
+  wp_pures.
+  wp_loadField.
+  wp_apply (KVClerk__Get_spec with "[$Hkck_own $Hks Hacc1_phys]"); first eauto.
+  iIntros (v_bal1_g) "Hbal1_get".
+  iDestruct "Hbal1_get" as (->) "[Hkck_own Hacc1_phys]".
+  wp_pures.
+  destruct bool_decide eqn:HenoughBalance; wp_pures.
+  - wp_loadField. wp_apply (KVClerk__Put_spec with "[$Hkck_own $Hks Hacc1_phys]"); first eauto.
+    iIntros "[Hkck_own Hacc1_phys]".
+    wp_pures.
+    wp_loadField.
+    wp_apply (KVClerk__Get_spec with "[$Hkck_own $Hks Hacc2_phys]"); first eauto.
+    iIntros (v_bal2_g) "Hbal2_get".
+    iDestruct "Hbal2_get" as (->) "[Hkck_own Hacc2_phys]".
+    wp_loadField.
+    wp_apply (KVClerk__Put_spec with "[$Hkck_own $Hks Hacc2_phys]"); first eauto.
+    iIntros "[Hkck_own Hacc2_phys]".
+    wp_pures.
+    iApply fupd_wp.
+    iInv bankN as ">HbankInv" "HbankInvClose".
+    iNamed "HbankInv".
+    iMod (map_update acc1 _ (word.sub bal1 amount) with "HlogBalCtx Hacc1_log") as "[HlogBalCtx Hacc1_log]".
+    iMod (map_update acc2 _ (word.add bal2 amount) with "HlogBalCtx Hacc2_log") as "[HlogBalCtx Hacc2_log]".
+    iMod ("HbankInvClose" with "[HlogBalCtx]") as "_".
+    { iNext. iExists _, _. iSplitL "HlogBalCtx".
+      - rewrite insert_union_l. rewrite insert_singleton. 
+        rewrite insert_union_r; last by apply lookup_singleton_ne. rewrite insert_singleton. 
+        iFrame.
+      - admit. (* FIXME: add the necessary overflow checks and use them here... *)
+    }
+    iModIntro.
+    wp_loadField.
+    wp_apply (release_two_spec with "[$Hlck_own $Hls Hacc1_phys Hacc2_phys Hacc1_log Hacc2_log]").
+    { iSplitL "Hacc1_phys Hacc1_log"; iExists _; iFrame. }
+    iIntros "Hlck_own".
+    iApply "Hpost".
+    iExists _, _, _, _; iFrame "∗ # %".
+  - wp_loadField. wp_apply (release_two_spec with "[$Hlck_own $Hls Hacc1_phys Hacc2_phys Hacc1_log Hacc2_log]").
+    { iSplitL "Hacc1_phys Hacc1_log"; iExists _; iFrame. }
+    iIntros "Hlck_own".
+    iApply "Hpost".
+    iExists _, _, _, _; iFrame "∗ # %".
 Admitted.
 
 End bank_proof.
